core/properties/surjectivity/surjectivity.v
@@ -30,7 +30,7 @@ forall (tr: Transformation) (sm : SourceModel) (te : TargetElementType),
       In te (execute tr sm).(modelElements) ->
       (exists (sp : InputPiece),
           In sp (allTuples tr sm) /\
-          In te (elements_proj (traceTrOnPiece tr sm sp))).
+          In te (produced_elements (traceTrOnPiece tr sm sp))).
 Proof.
     apply tr_execute_in_elements.
 Qed.
