transformations/Families2Persons/theorems/sampleTheorems.v
@@ -16,7 +16,7 @@ Theorem tr_FamiliesToPersons :
       (exists (se : FamiliesMetamodel_Object),
           In se sm.(modelElements) /\
           In te
-            (elements_proj (traceTrOnPiece Families2Persons sm [se]))).
+            (produced_elements (traceTrOnPiece Families2Persons sm [se]))).
 Proof.
     intros.
     apply (tr_execute_in_elements Families2Persons) in H.
